Generic struct support (#243)
Companion to goose-lang/goose#92 providing some additional/fixed automation and updating translations.

I made one tweak to help with generic types where all Settable instances explicitly specify the type, hence why all the translations are affected, but otherwise non-generic types are translated identically to before.

new/etc/update-goose-new.py
@@ -259,7 +259,7 @@ def main():
             path.join(goose_dir, "testdata/examples"),
             "./append_log",
             "./semantics",
-            "./unittest",
+            "./unittest/...",
         )
 
     if args.std_lib:
