new/generatedproof/go_etcd_io/etcd/api/v3/mvccpb.v
@@ -37,7 +37,7 @@ End KeyValue.
 Section instances.
 Context `{ffi_syntax}.
 
-Global Instance settable_KeyValue : Settable _ :=
+Global Instance settable_KeyValue : Settable KeyValue.t :=
   settable! KeyValue.mk < KeyValue.Key'; KeyValue.CreateRevision'; KeyValue.ModRevision'; KeyValue.Version'; KeyValue.Value'; KeyValue.Lease'; KeyValue.XXX_NoUnkeyedLiteral'; KeyValue.XXX_unrecognized'; KeyValue.XXX_sizecache' >.
 Global Instance into_val_KeyValue : IntoVal KeyValue.t :=
   {| to_val_def v :=
@@ -159,7 +159,7 @@ End Event.
 Section instances.
 Context `{ffi_syntax}.
 
-Global Instance settable_Event : Settable _ :=
+Global Instance settable_Event : Settable Event.t :=
   settable! Event.mk < Event.Type'; Event.Kv'; Event.PrevKv'; Event.XXX_NoUnkeyedLiteral'; Event.XXX_unrecognized'; Event.XXX_sizecache' >.
 Global Instance into_val_Event : IntoVal Event.t :=
   {| to_val_def v :=
