new/generatedproof/go_etcd_io/etcd/client/v3/leasing.v
@@ -37,7 +37,7 @@ End leaseCache.
 Section instances.
 Context `{ffi_syntax}.
 
-Global Instance settable_leaseCache : Settable _ :=
+Global Instance settable_leaseCache : Settable leaseCache.t :=
   settable! leaseCache.mk < leaseCache.mu'; leaseCache.entries'; leaseCache.revokes'; leaseCache.header' >.
 Global Instance into_val_leaseCache : IntoVal leaseCache.t :=
   {| to_val_def v :=
@@ -121,7 +121,7 @@ End leaseKey.
 Section instances.
 Context `{ffi_syntax}.
 
-Global Instance settable_leaseKey : Settable _ :=
+Global Instance settable_leaseKey : Settable leaseKey.t :=
   settable! leaseKey.mk < leaseKey.response'; leaseKey.rev'; leaseKey.waitc' >.
 Global Instance into_val_leaseKey : IntoVal leaseKey.t :=
   {| to_val_def v :=
@@ -205,7 +205,7 @@ End leasingKV.
 Section instances.
 Context `{ffi_syntax}.
 
-Global Instance settable_leasingKV : Settable _ :=
+Global Instance settable_leasingKV : Settable leasingKV.t :=
   settable! leasingKV.mk < leasingKV.cl'; leasingKV.kv'; leasingKV.pfx'; leasingKV.leases'; leasingKV.ctx'; leasingKV.cancel'; leasingKV.wg'; leasingKV.sessionOpts'; leasingKV.session'; leasingKV.sessionc' >.
 Global Instance into_val_leasingKV : IntoVal leasingKV.t :=
   {| to_val_def v :=
@@ -334,7 +334,7 @@ End txnLeasing.
 Section instances.
 Context `{ffi_syntax}.
 
-Global Instance settable_txnLeasing : Settable _ :=
+Global Instance settable_txnLeasing : Settable txnLeasing.t :=
   settable! txnLeasing.mk < txnLeasing.Txn'; txnLeasing.lkv'; txnLeasing.ctx'; txnLeasing.cs'; txnLeasing.opst'; txnLeasing.opse' >.
 Global Instance into_val_txnLeasing : IntoVal txnLeasing.t :=
   {| to_val_def v :=
