new/should_build.v
@@ -1,5 +1,6 @@
 From New.code.go_etcd_io.raft Require v3.
-From New.code.github_com.goose_lang.goose.testdata.examples Require unittest semantics.
+From New.generatedproof.github_com.goose_lang.goose.testdata.examples
+  Require unittest unittest.generics semantics.
 (* required just to make sure this demo works *)
 From New.golang.theory Require static_mem.
 From New.proof Require go_etcd_io.etcd.raft.v3.
